adding another primitive to UInt* (mul_div)

ulib/FStar.UInt.fst
@@ -149,6 +149,12 @@ val mul_mod: #n:nat -> a:uint_t n -> b:uint_t n -> Tot (uint_t n)
 let mul_mod #n a b =
   (a * b) % (pow2 n)
 
+val mul_div: #n:nat -> a:uint_t n -> b:uint_t n -> Tot (uint_t n)
+#reset-options "--max_fuel 0 --max_ifuel 0"
+let mul_div #n a b =
+  FStar.Math.Lemmas.lemma_mult_lt_sqr a b (pow2 n);
+  (a * b) / (pow2 n)
+
 (* Division primitives *)
 val div: #n:nat -> a:uint_t n -> b:uint_t n{b <> 0} -> Pure (uint_t n)
   (requires (size (a / b) n))
